# FUNKCIJE

## VRSTE TRIGONOMETRIČNIH FUNKCIJ
### Sinus
$\sin{x} = \alpha$

$x = ?$, $\alpha \in [-1, 1]$

$x_1 = \arcsin{\alpha} + 2k \pi$   $k \in \mathbb{Z}$

$x_2 = (\pi - x_1) + 2k\pi$

#### Posebni primeri
1. $\sin{x} = 0$ -> $x = k*\pi$     $k \in \mathbb{Z}$

2. $\sin{x} = 1$ -> $x_{max} = \frac{\pi}{2} + 2k*\pi$     $k \in \mathbb{Z}$

3. $\sin{x} = -1$ -> $x_{min} = -\frac{\pi}{2} + 2k*\pi$     $k \in \mathbb{Z}$

### Cosinus
$\cos{x} = \alpha$

$x = ?$, $\alpha \in [-1, 1]$

$x_1 = \arccos{b} + 2k\pi$   $k \in \mathbb{Z}$

$x_2 = -x_1 + 2k\pi$
#### Posebni primeri
1. $\cos{x} = 0$ -> $x_0 = \frac{\pi}{2} + k\pi$   $k \in \mathbb{Z}$

2. $\cos{x} = 1$ -> $x_{max} = 2k * \pi$   $k \in \mathbb{Z}$    

3. $\cos{x} = −1$ -> $x_{min} = (2k - 1) * \pi$   $k \in \mathbb{Z}$

### Tangens
$\tan{x} = c$

$x = \arctan{c} + k\pi$   $k \in \mathbb{Z}$


### Cotangens
$\cot{x} = d \rightarrow \tan{x} = \frac{1}{d}$

$x = \arctan{\frac{1}{d}} + k\pi$   $k \in \mathbb{Z}$

## METODA POLOVIČNIH KOTOV


## HOMOGENE TRIGONOMETRIČNE ENAČBE 2. STOPNJE

$a*\sin²{x} + b*\sin{x} * \cos{x} + c*\cos²{x} = 0$

->

$\frac{a*\sin²{x}}{\cos²{x}} + \frac{b*\sin{x}}{\cos{x}} + c = 0$

->

$a*\tan²{x} + b*\tan{x} + c = 0$

# DEFINICIJE FUNKCIJ
$\sin{\alpha} = \frac{nasprotna kateta}{hipotenuza} = \frac{a}{c}$

$\cos{\alpha} = \frac{priležna kateta}{hipotenuza} = \frac{b}{c}$

$\tan{\alpha} = \frac{nasptronta kateta}{priležna kateta} = \frac{a}{b}$ tudi $\tan{\alpha} = \frac{\sin{\alpha}}{\cos{\alpha}}$

$\cot{\alpha} = \frac{priležna kateta}{nasprotna kateta} = \frac{b}{a}$ tudi $\cot{\alpha} = \frac{\cos{\alpha}}{\sin{\alpha}}$ ali pa $\cot{\alpha} = (\tan{\alpha})^{-1}$


## Pomembne enačbe
$\sin{(2\alpha)} = 2 * sin{\alpha} * \cos{\alpha}$

$\cos{(2\alpha)} = \cos^{2}\left(\alpha\right) - \sin^{2}\left(\alpha\right)$

$\sin^{2}\left(\alpha\right) + \cos^{2}\left(\alpha\right) = 1$


$\sin{(\alpha + \beta)} = \sin{\alpha} * \cos{\beta} + \sin{\beta} * \cos{\alpha}$

$\sin{(\alpha - \beta)} = \sin{\alpha} * \cos{\beta} + \sin{\beta} * \cos{\alpha}$


$\cos{(\alpha + \beta)} = \cos{\alpha} * \cos{\beta} - \sin{\alpha} * \sin{\beta}$

$\cos{(\alpha - \beta)} = \cos{\alpha} * \cos{\beta} + \sin{\alpha} * \sin{\beta}$